% Exercise 1.1
\begin{exercise}

Prove \textit{de Morgan's law}:

\[ (A \cup B)^c = A^c \cap B^c \]

and

\[ (A \cap B)^c = A^c \cup B^c \]

both directly and using indicator functions.

\end{exercise}
\begin{solution}

Let's prove $(A\cup B)^c = A^c\cap B^c$, then $(A \cap B)^c = A^c \cup B^c$ can be proved in a similar way.\\

\textit{Directly}

$\subseteq$ - For an element $x\in(A\cup B)^c$, then $x\notin A\cup B=\{ y | y\in A \vee y\in B \}$. In this case, $x\notin A$ and $x\notin B$, that is $x\in A^c$ and $x\in B^c$. Hence, $x\in A^c\cap B^c$. Given that this holds for all $x\in(A\cup B)^c$, we have $(A\cup B)^c \subseteq A^c\cap B^c$.

$\supseteq$ - For an element $x\in A^c\cap B^c$, it means $x\in A^c$ and $x\in B^c$. In this case, $x\notin A$ and $x\notin B$, hence $x\notin A\cup B$ by definition. Therefore, $x\in (A\cup B)^c$. Given that this holds for all $x\in A^c\cap B^c$, we have $(A\cup B)^c \supseteq A^c\cap B^c$.\\

\textit{Indicator functions}
\begin{align*}
\dsone_{(A\cup B)^c} &= 1 - \dsone_{A\cup B} \\
  &= 1 - \max\{ \dsone_A, \dsone_B \} \\
  &= \min\{ 1-\dsone_A, 1-\dsone_B \} \\
  &= \min\{ \dsone _{A^c}, \dsone _{B^c} \} \\
  &= \dsone _{A^c\cap B^c}
\end{align*}

\end{solution}


% Exercise 1.2
\begin{exercise}

Prove that for events $A$ and $B$, $A\Delta B = A^c \Delta B^c$.

\end{exercise}
\begin{solution}

By definition
\begin{align*}
A\Delta B &= A\setminus B + B\setminus A \\
  &= A\cap B^c + B\cap A^c \\
  &= A^c \cap (B^c)^c + B^c \cap (A^c)^c \\
  &= A^c\setminus B^c + B^c\setminus A^c \\
  &= A^c\Delta B^c
\end{align*}

\end{solution}

\newpage
% Exercise 1.3
\begin{exercise}

Let $B$ and $C$ be events $(A_n)$ and let $A_n=B$ if $n$ is odd and $A_n=C$ if $n$ is even. Calculate $\limsup_{n} A_n$ and $\liminf_{n} A_n$.

\end{exercise}
\begin{solution}

Intuitively while $n$ goes to $\infty$, $\limsup_{n} A_n$ is the set where $A_n$ will \textit{``never leave forever''}, and $\liminf_{n} A_n$ is the set where $A_n$ will \textit{``eventually stay forever''}. Since $A_n$ is alternating between $B$ and $C$, $\limsup_{n} A_n = B\cup C$ and $\liminf_{n} A_n = B\cap C$. \\

Now, let's prove it. By definition
\begin{align*}
\limsup_n A_n &= \bigcap_{k=1}^\infty\bigcup_{n=k}^\infty A_n \\
  &= \bigcap_{k=1}^\infty(\bigcup_{n=2k-1}^{\infty}A_n\cup \bigcup_{n=2k}^{\infty}A_n\big) \\
  &= \bigcap_{k=1}^\infty (B\cup C) \\
  &= B \cup C
\end{align*}
And
\begin{align*}
\liminf_n A_n &= \bigcup_{k=1}^\infty\bigcap_{n=k}^\infty A_n \\
  &= \bigcup_{k=1}^\infty(\bigcap_{n=2k-1}^{\infty}A_n\cap \bigcap_{n=2k}^{\infty}A_n\big) \\
  &= \bigcup_{k=1}^\infty (B\cap C) \\
  &= B \cap C
\end{align*}

\end{solution}


% Exercise 1.4
\begin{exercise}
Prove part b) of proposition 1.9: Let $A_1,A_2,\ldots$ be subsets of $\Omega$. If $A_1\supseteq A_2\supseteq \cdots$, then $A_n\to A=\cap_{n=1}^\infty A_n$. (This is written as $A_n\downarrow A$)
\end{exercise}
\begin{solution}
Let $A=\cap_{n=1}^\infty A_n$. To prove $A_n\to A$, we can show 1) $\liminf_n A_n = A$, and 2) $\limsup_n A_n = A$. \\

1) Given $A_1\supseteq A_2\supseteq \cdots$, for each $k$, $\cap_{n=k}^\infty A_n=A$. Hence by definition

\[ \liminf_n A_n = \bigcup_{k=1}^\infty\bigcap_{n=k}^\infty A_n=\bigcup_{k=1}^\infty A = A .\]

2) On the other hand, for each $k$, $\cup_{n=k}^\infty A_n = A_k$, by definition

\[ \limsup_n A_n = \bigcap_{k=1}^\infty\bigcup_{n=k}^\infty A_n = \bigcap_{k=1}^\infty A_k = A .\]

\end{solution}


% Exercise 1.5
\begin{exercise}
Prove that \\
a) if $t_n\downarrow t$, then $(-\infty, t_n]\downarrow (-\infty, t]$, but that \\
b) if $t_n\uparrow t$ and $t_n < t$ for each $n$, then $(-\infty, t_n]\uparrow (-\infty, t)$.
\end{exercise}
\begin{solution}
Let's prove a), then b) can be proved in a similar way. By Proposition 1.9,

\[(-\infty, t_n] \downarrow \bigcap_{n=1}^\infty (-\infty, t_n] .\]

It is left to show that $\cap_{n=1}^\infty(-\infty, t_n] = (-\infty, t]$. \\

Let $x\in\cap_{n=1}^\infty(-\infty, t_n]$, then $x\leq t_n$ for all $n$. As $n\to\infty$, $t_n\to t$ and $x \leq t$, so $x\in (-\infty, t]$. On the other hand, if $x\in(-\infty, t]$, then $x\leq t\leq t_n$ for all $n$. Therefore, we have $\cap_{n=1}^\infty(-\infty, t_n] = (-\infty, t]$.
\end{solution}