# Chapter 1. Probability

## Exercise 1.6
Show that the disjointification procedure used to prove Proposition 1.24 actually yields $\cup_{n=1}^k A_n=\Sigma_{n=1}^k B_n$ for every $k$.

### Solution

Let $k=1$, then $A_1=B_1$. Assume $\cup_{n=1}^k A_n=\Sigma_{n=1}^k B_n$ holds for some $k>1$, then
$$\begin{align*}
\cup_{n=1}^{k+1} A_n &= A_{k+1}\cup (\cup_{n=1}^{k} A_n) \\
  &= (A_{k+1}\backslash\cup_{n=1}^{k} A_n) + \cup_{n=1}^{k} A_n \\
  &= B_{k+1} + \Sigma_{n=1}^k B_n \\
  &= \Sigma_{n=1}^{k+1} B_n
\end{align*}$$
Therefore, the statement is proved by induction.

